SetTheory/lean/SetTheory/Audit.lean
@@ -265,6 +265,8 @@ open SetTheory
 #check @PA.Formula.BProv_Ax_s_remAt_of_eqConst
 #check @PA.Formula.BProv_Ax_s_remAt_constMod_of_eqConst
 #check @PA.Formula.BProv_Ax_s_remAt_constRemMod_of_eqConst
+#check @PA.Formula.BProv_Ax_s_ltAt_of_remAt
+#check @PA.Formula.BProv_Ax_s_remEqAt_of_remAt
 #check @PA.Formula.BProv_Ax_s_betaModTerm_of_eqConst
 #check @PA.Formula.BProv_Ax_s_betaAt_of_eqConst
 #check @PA.Formula.BProv_Ax_s_betaAt_constOutSubst_of_eqConst
